finish SimpleWhileCompletness

SimpleWhile/SimpleWhileCompletness.v
@@ -23,6 +23,73 @@ Import Lang_SimpleWhile
        HoareSimpleWhile_Derived
        HoareSimpleWhile_Admissible.
 
+Definition wp (c:com) (Q:assertion) : assertion :=
+  fun s => forall s', eval_com c s s' -> Q s'.
+
+Hint Unfold wp : core.
+
+Theorem wp_is_precondition : forall c Q,
+  valid {{wp c Q}} c {{Q}}.
+Proof.
+  intros.
+  unfold valid.
+  intros s1 s2.
+  unfold wp.
+  intros.
+  apply H.
+  tauto.
+Qed.
+
+Theorem wp_is_weakest : forall c Q P',
+    valid {{P'}} c {{Q}} ->
+    P' |-- (wp c Q).
+Proof.
+  unfold valid.
+  unfold derives.
+  unfold wp.
+  intros.
+  specialize (H s s').
+  apply H; tauto.
+Qed.
+
+Lemma wp_seq : forall P Q c1 c2,
+    provable {{P}} c1 {{(wp c2 Q)}} -> 
+    provable {{(wp c2 Q)}} c2 {{Q}} -> provable {{P}} [[c1; c2]] {{Q}}.
+Proof.
+  intros.
+  eapply hoare_seq; [apply H|apply H0].
+Qed.
+
+Lemma wp_invariant : forall b c Q,
+    valid {{ (wp (CWhile b c) Q) && [[ b ]] }} c {{ wp (CWhile b c) Q }}.
+Proof.
+  unfold valid.
+  unfold wp.
+  assn_unfold.
+  intros.
+  destruct H.
+  specialize (H s').
+  apply H.
+  revert H1 H2 H0.
+  simpl.
+  unfold while_sem.
+  unfold_RELS_tac.
+  intros.
+  destruct H1.
+  exists (S x).
+  simpl.
+  unfold_RELS_tac.
+  exists s1.
+  split.
+  + unfold test_true.
+    unfold_RELS_tac.
+    split; [|tauto].
+    revert H2.
+    unfold eb2assn. tauto.
+  + exists s2.
+    tauto.
+Qed.
+
 Theorem hoare_complet: forall P Q c,
    valid {{ P }} c {{ Q }} -> provable {{ P }} c {{ Q }}.
 Proof.
@@ -61,7 +128,20 @@ Proof.
     destruct (x =? Y)%string eqn : I; auto.
     apply String.eqb_eq in I.
     rewrite I in H3; contradiction.
-  + admit.
+  + apply (hoare_seq P (fun s => exists x: state, P x /\ eval_com c1 x s) Q).
+    - apply IHc1.
+      intros.
+      exists s1.
+      tauto.
+    - apply IHc2.
+      intros.
+      destruct H,H.
+      specialize (HT x s2).
+      apply HT; [tauto|].
+      simpl.
+      unfold seq_sem.
+      unfold_RELS_tac.
+      exists s1; tauto.
   + apply hoare_if.
     - specialize (IHc1 Assn(P && [[e]]) Q).
       apply IHc1.
@@ -97,9 +177,36 @@ Proof.
         intros.
         unfold negb in H; destruct H.
         destruct (eval_expr_bool e s1); auto.
-  +  
-        
-        
-        
-
+  + pose proof wp_invariant e c Q.
+    specialize (IHc  Assn((wp (CWhile e c) Q) && [[e]])  (wp (CWhile e c) Q)).
+    unfold valid in H.
+    apply IHc in H.
+    apply hoare_while in H.
+    eapply hoare_conseq; [apply H| |].
+    - unfold derives.
+      unfold wp.
+      intros. 
+      specialize (HT s s').
+      tauto.
+    - unfold derives.
+      unfold wp.
+      assn_unfold.
+      intros.
+      destruct H0.
+      specialize (H0 s).
+      apply H0.
+      simpl.
+      revert H1.
+      unfold while_sem.
+      unfold_RELS_tac.
+      unfold eb2assn.
+      simpl.
+      unfold not_sem.
+      unfold negb.
+      intros.
+      exists O. simpl.
+      unfold test_false.
+      unfold_RELS_tac.
+      split; [|tauto].
+      destruct (eval_expr_bool e s); auto.
 Qed.
